src/paths/Some_lemmas.v
@@ -87,6 +87,156 @@ Proof.
   introv Hr. rewrite open_var_path_typ_eq. apply* open_record_type_p.
 Qed.
 
+Lemma open_fresh_avar_injective : forall x y k z,
+    z \notin fv_avar x ->
+    z \notin fv_avar y ->
+    open_rec_avar k z x = open_rec_avar k z y ->
+    x = y.
+Proof.
+  intros. destruct x, y; inversion H1.
+  - case_if.
+    + case_if. subst. reflexivity.
+    + case_if. assumption.
+  - case_if. simpl in H0. inversions H3. false* notin_same.
+  - case_if. simpl in H. inversions H3. false* notin_same.
+  - reflexivity.
+Qed.
+
+Lemma open_fresh_typ_dec_injective:
+  (forall T T' k x,
+    x \notin fv_typ T ->
+    x \notin fv_typ T' ->
+    open_rec_typ k x T = open_rec_typ k x T' ->
+    T = T') /\
+  (forall D D' k x,
+    x \notin fv_dec D ->
+    x \notin fv_dec D' ->
+    open_rec_dec k x D = open_rec_dec k x D' ->
+    D = D') /\
+  (forall p p' k x,
+      x \notin fv_path p ->
+      x \notin fv_path p' ->
+      open_rec_path k x p = open_rec_path k x p' ->
+      p = p').
+Proof.
+  apply typ_mutind; intros.
+  - destruct T'; inversions H1. reflexivity.
+  - destruct T'; inversions H1. reflexivity.
+  - destruct T'; inversions H2. apply f_equal. apply* (H d0 k x).
+  - destruct T'; inversions H3.
+    assert (t = T'1). {
+      apply (H T'1 k x).
+      - simpl in H1. auto.
+      - simpl in H2. auto.
+      - assumption.
+    }
+    assert (t0 = T'2). {
+      apply (H0 T'2 k x).
+      - simpl in H1. auto.
+      - simpl in H2. auto.
+      - assumption.
+    }
+    subst*.
+  - destruct T'; inversions H2. simpls. specialize (H _ _ _ H0 H1 H4). subst*.
+  - destruct T'; inversions H2.
+    apply f_equal. apply (H T' (Datatypes.S k) x).
+    + simpl in H. assumption.
+    + simpl in H0. assumption.
+    + assumption.
+  - destruct T'; inversions H3.
+    assert (t = T'1). {
+      apply (H T'1 k x).
+      - simpl in H1. auto.
+      - simpl in H2. auto.
+      - assumption.
+    }
+    assert (t0 = T'2). {
+      apply (H0 T'2 (S k) x).
+      - simpl in H1. auto.
+      - simpl in H2. auto.
+      - assumption.
+    }
+    subst*.
+  - destruct T'; inversions H2. specialize (H _ _ _ H0 H1 H4). subst*.
+  - destruct D'; inversions H3.
+    assert (t0 = t3). {
+      apply (H t3 k x).
+      - simpl in H1. auto.
+      - simpl in H2. auto.
+      - assumption.
+    }
+    assert (t1 = t4). {
+      apply (H0 t4 k x).
+      - simpl in H1. auto.
+      - simpl in H2. auto.
+      - assumption.
+    }
+    subst*.
+  - destruct D'; inversions H2.
+    apply f_equal. apply (H t2 k x).
+    + simpl in H0. assumption.
+    + simpl in H1. assumption.
+    + assumption.
+  - destruct p'; inversions H1.
+    lets Hx: (open_fresh_avar_injective _ _ _ H H0 H3). subst*.
+  - destruct p'; inversions H2.
+    simpls. specialize (H _ _ _ H0 H1 H4). subst*.
+Qed.
+
+Lemma opening_preserves_labels : forall z T ls ls',
+    record_typ T ls ->
+    record_typ (open_typ z T) ls' ->
+    ls = ls'.
+Proof.
+  introv Ht Hopen. gen ls'.
+  dependent induction Ht; intros.
+  - inversions Hopen. rewrite open_var_path_dec_eq.
+    rewrite open_dec_preserves_label with (x:=p_var (avar_f z)) (i:=0).
+    unfold open_dec_p. reflexivity.
+  - inversions Hopen. rewrite open_var_path_dec_eq.
+    rewrite open_dec_preserves_label with (x:=p_var (avar_f z)) (i:=0).
+    specialize (IHHt ls0 H4). rewrite* IHHt.
+Qed.
+
+Lemma record_type_open : forall z T,
+    z \notin fv_typ T ->
+    record_type (open_typ z T) ->
+    record_type T.
+Proof.
+  introv Hz H. destruct H. dependent induction H.
+  - exists \{ l }. destruct T; inversions x. constructor.
+    + destruct d; inversions H.
+      * apply (proj21 open_fresh_typ_dec_injective) in H3.
+        { subst. constructor. }
+        { simpl in Hz; auto. }
+        { simpl in Hz; auto. }
+      * constructor.
+    + destruct d; inversions H.
+      * apply (proj21 open_fresh_typ_dec_injective) in H3.
+        { subst. constructor. }
+        { simpl in Hz; auto. }
+        { simpl in Hz; auto. }
+      * constructor.
+  - destruct T; inversions x. simpl in Hz.
+    assert (Hz': z \notin fv_typ T1) by auto.
+    destruct (IHrecord_typ T1 z Hz' eq_refl) as [ls' ?]. clear Hz'.
+    destruct T2; inversions H5.
+    destruct d; inversions H0.
+    + exists (ls' \u \{ label_typ t }). apply (proj21 open_fresh_typ_dec_injective) in H6.
+      * subst. constructor*.
+        { constructor. }
+        {
+          simpl in H2. pose proof (opening_preserves_labels z H1 H).
+          rewrite* H0.
+        }
+      * simpl in Hz; auto.
+      * simpl in Hz; auto.
+    + exists (ls' \u \{ label_trm t }). constructor*.
+      * constructor.
+      * simpl in H2. pose proof (opening_preserves_labels z H1 H).
+        rewrite* H0.
+Qed.
+
 (* ###################################################################### *)
 (** *** Lemmas about Record has *)
 
@@ -244,4 +394,36 @@ Proof.
   - exists E (@empty A). rewrite concat_empty_r. reflexivity.
   - apply binds_push_neq_inv in Hb. destruct (IHE Hb) as [E' [E'' HE]]. subst.
     exists E' (E'' & x0 ~ v0). rewrite concat_assoc. reflexivity. assumption.
+Qed.
+
+Lemma hasnt_notin : forall G z T ds ls t U,
+    G && z ~ T |- ds :: U ->
+    record_typ U ls ->
+    defs_hasnt ds t ->
+    t \notin ls.
+Proof.
+  introv Hds Hrec Hhasnt.
+  inversions Hhasnt. gen ds. induction Hrec; intros.
+  - inversions Hds. inversions H7; simpl in *; case_if; apply* notin_singleton.
+  - apply notin_union; split.
+    + inversions Hds. apply (IHHrec ds0 H5). simpl in *. case_if*.
+    + inversions Hds. inversions H10; simpl in *; case_if; apply* notin_singleton.
+Qed.
+
+Lemma ty_defs_record_type : forall G z U ds T,
+    G && z ~ U |- ds :: T ->
+    record_type T.
+Proof.
+  intros.
+  dependent induction H.
+  - destruct D.
+    + inversions H. exists \{ label_typ t }. constructor*. constructor.
+    + exists \{ label_trm t }. constructor*. constructor.
+  - destruct IHty_defs. destruct D.
+    + unfold record_type. exists (x0 \u \{ label_typ t }). constructor*.
+      * inversions H0. constructor.
+      * inversions H0. simpl in H1. apply (hasnt_notin H H2 H1).
+    + exists (x0 \u \{ label_trm t }). constructor*.
+      * constructor.
+      * inversions H0; simpl in H1; apply (hasnt_notin H H2 H1).
 Qed.
